code/hash/Hacl.SHA2Again.fst
@@ -1,0 +1,37 @@
+module Hacl.SHA2Again
+
+module U32 = FStar.UInt32
+module U64 = FStar.UInt64
+module C = Spec.SHA2Again.Constants
+module S = FStar.Seq
+module B = LowStar.Buffer
+module HS = FStar.HyperStack
+module ST = FStar.HyperStack.ST
+
+friend Spec.SHA2Again
+
+// 20180809 bug: need to start interactive mode with nothing beyond this line, then load the rest
+module Spec = Spec.SHA2Again
+
+let h224 = B.gcmalloc_of_list HS.root C.h224_l
+let h256 = B.gcmalloc_of_list HS.root C.h256_l
+let h384 = B.gcmalloc_of_list HS.root C.h384_l
+let h512 = B.gcmalloc_of_list HS.root C.h512_l
+
+let k224_256 = B.gcmalloc_of_list HS.root C.k224_256_l
+let k384_512 = B.gcmalloc_of_list HS.root C.k384_512_l
+
+let hashes a s l =
+  Spec.hashes a s l
+
+let init a =
+  C.h224_reveal ();
+  C.h256_reveal ();
+  C.h384_reveal ();
+  C.h512_reveal ();
+  let l: list (word a) = Spec.(match a with
+    | SHA2_224 -> C.h224_l
+    | SHA2_256 -> C.h256_l
+    | SHA2_384 -> C.h384_l
+    | SHA2_512 -> C.h512_l) in
+  B.alloca_of_list l
