code/hash/Hacl.SHA2Again.fsti
@@ -1,0 +1,36 @@
+module Hacl.SHA2Again
+
+module U32 = FStar.UInt32
+module U64 = FStar.UInt64
+module C = Spec.SHA2Again.Constants
+module S = FStar.Seq
+module B = LowStar.Buffer
+module HS = FStar.HyperStack
+module ST = FStar.HyperStack.ST
+module M = LowStar.Modifies
+
+module Spec = Spec.SHA2Again
+
+(** Lifting words, state and abstract predicates in the stateful style. *)
+
+let word a =
+  let open Spec in
+  match a with
+  | SHA2_224 | SHA2_256 -> U32.t
+  | SHA2_384 | SHA2_512 -> U64.t
+
+type state a =
+  b:B.buffer (word a) { B.length b = Spec.size_hash_w }
+
+val hashes: a:Spec.hash_alg ->
+  (s: S.seq (word a) { S.length s = Spec.size_hash_w }) ->
+  (l:Spec.bytes_blocks a) ->
+  Type0
+
+val init: a:Spec.hash_alg -> ST.StackInline (state a)
+  (requires (fun h ->
+    HS.is_stack_region (HS.get_tip h)))
+  (ensures (fun h0 s h1 ->
+    M.(modifies M.loc_none h0 h1) /\
+    B.live h1 s /\
+    hashes a (B.as_seq h1 s) S.empty))
